<section xml:id="sec_implicit_functions_tutorial">
  <title>Implicit Functions</title>
  <p>
    An implicit function cannot be defined as a normal function.
    Instead, the curve is defined as an
    <em>equation</em> of multiple variables.
    It is easiest to assign a name to the entire equation,
    including the <m>=</m> sign.
  </p>
  <p>
    \begin{maplegroup} \begin{mapleinput} {E := y\symbol{94}2 = x\symbol{94}3 - 2*x + 1; } \end{mapleinput} \relax \begin{maplelatex} {E := y^2 = x^3-2*x+1}{
    <me>
      \displaystyle E\, := \,{y}^{2}={x}^{3}-2\,x+1
    </me>
  </p>
  <p>
    } \end{maplelatex} \end{maplegroup}
  </p>
  <p>
        <idx><h>subs</h></idx>
        <idx><h>solving equations</h><h>solve</h></idx>
        <idx><h>ditto operator</h></idx>
  </p>
  <p>
    To find points on the curve,
    we can substitute a value for <m>x</m> and solve for <m>y</m>.
  </p>
  <p>
    \begin{maplegroup} \begin{mapleinput} {subs(x=2, E); } \end{mapleinput} \relax \begin{maplelatex} {y^2 = 5}{
    <me>
      \displaystyle {y}^{2}=5
    </me>
  </p>
  <p>
    } \end{maplelatex} \end{maplegroup}
  </p>
  <p>
    \begin{maplegroup} \begin{mapleinput} {solve( } \end{mapleinput} \relax \begin{maplelatex} {sqrt(5), -sqrt(5)}{
    <me>
      \displaystyle  \sqrt{5},\,- \sqrt{5}
    </me>
  </p>
  <p>
    } \end{maplelatex} \end{maplegroup}
  </p>
  <p>
    Many implicit functions cannot be expressed as a single function <m>y=f(x)</m>.
    However, it may be possible to split up implicit functions into explicit functions by solving for <m>y</m>.
  </p>
  <p>
    <idx><h>mathematical functions</h><h>nth root@<m>n</m><sup>th</sup> root</h></idx>
  </p>
  <p>
    \begin{maplegroup} \begin{mapleinput} {L := x\symbol{94}2 + (y - root[3](x\symbol{94}2))\symbol{94}2 = 1; } \end{mapleinput} \relax \begin{maplelatex} {L := x^2+(y-(x^2)^(1/3))^2 = 1}{
    <me>
      \displaystyle L\, := \,{x}^{2}+ \left( y-\sqrt [3]{{x}^{2}} \right) ^{2}=1
    </me>
  </p>
  <p>
    } \end{maplelatex} \end{maplegroup}
  </p>
  <aside>
    <p>
      Here, the command <c>root[3]()</c> is equivalent to <m>\sqrt[3]{(~)}</m>.
    </p>
  </aside>
  <p>
    \begin{maplegroup} \begin{mapleinput} {solve(L, y); } \end{mapleinput} \relax \begin{maplelatex} {(x^2)^(1/3)+sqrt(-x^2+1), (x^2)^(1/3)-sqrt(-x^2+1)}{
    <me>
      \displaystyle \sqrt [3]{{x}^{2}}+ \sqrt{-{x}^{2}+1},\,\sqrt [3]{{x}^{2}}- \sqrt{-{x}^{2}+1}
    </me>
  </p>
  <p>
    } \end{maplelatex} \end{maplegroup}
  </p>
</section>